# Differenciation

## Derivative of a Constant Rule
Let $c$ be a constant
then,
$$
c' = 0
$$

## Constant Multiple Rule
Let $c$ be a constant
then,
$$
{\bigl( c \cdot f(x) \bigr)}' = c \cdot f'(x)
$$

## Sum/Difference Rule
Let $f'(x)$ and $g'(x)$ exist
then,
$$
{\bigl( f(x) \pm g(x) \bigr)}' = f'(x) \pm g'(x)
$$

## Product Rule
Let $f'(x)$ and $g'(x)$ exist
then,
$$
{\bigl( f(x) \cdot g(x) \bigr)}' = f'(x) \cdot g(x) + f(x) \cdot g'(x)
$$

## Quotient Rule
Let $f'(x)$ and $g'(x)$ exist
then,
$$
{\left( \frac{f(x)}{g(x)} \right)}' = \frac{f'(x) \cdot g(x) - f(x) \cdot g'(x)}{{g(x)}^2}
$$

## Power Rule
Let $n \in \R$
then,
$$
{\left( x^n \right)}' = nx^{n-1}
$$

## Exponential Rule
Let $n \in \R$
then,
$$
{\left(n^x\right)}' = n^x \cdot \ln n
$$

## Chain Rule
Let $f'(x)$ and $g'(x)$ exist
then ${(f(g(x)))}'$ exists and,
$$
{\Bigl(f\bigl(g(x)\bigr)\Bigr)}' = f'\bigl(g(x)\bigr) \cdot g'(x)
$$

### Power + Chain Rule
$$
{\left( u^n \right)}' = n \cdot u^{n-1} \cdot u'
$$

## misc.
$$
\begin{align*}
    \log\left(a \cdot b\right) &= \log a + \log b \\
    \log\left(\frac{a}{b}\right) &= \log a - \log b \\
    \log{a^b} &= b \cdot \log a \\~\\
    x &= e^{\ln x} \\
    a &= e^{\ln a} \\
    a^x &= {(e^{\ln a})}^x \\
    a^x &= e^{(\ln a)x}
\end{align*}
$$
